cleanup

Constellation/ProcessRuleMutual.lean
@@ -10,21 +10,25 @@ abbrev Atom := Char
 abbrev PersistentName := String
 abbrev  EphemeralName := String
 
+abbrev PersistentNames := Finset PersistentName
+
 inductive Name where
   | Persistent: PersistentName → Name
   | Ephemeral :  EphemeralName → Name
 
 inductive Process: Type where
-  | par  (p₁ p₂: Process)
-  | seq  (p₁ p₂: Process)
-  | trig (n: EphemeralName)
-  | add  (n: PersistentName)
-  | rem  (n: PersistentName)
+  | par   (p₁ p₂: Process)
+  | trig  (n: EphemeralName)
+  | add   (n: PersistentName)
+  | rem   (n: PersistentName)
+  | later (p: Process)
+  | halt
+deriving BEq
 
 structure ReactiveRule: Type where
   name  : EphemeralName
-  guard : PersistentName
-  effect: Process
+  guard : PersistentNames
+  effect: List Process
 
 structure DeclRule: Type where
   antecedents: Finset PersistentName
@@ -32,12 +36,8 @@ structure DeclRule: Type where
 
 structure Program: Type where
   decl: Finset DeclRule
-  reac: Finset ReactiveRule
+  reac: List ReactiveRule
 
-abbrev Pending := List Process
-abbrev Persisting := Finset PersistentName
-
-abbrev PersistentNames := Finset PersistentName
 
 namespace DeclRule
 
@@ -55,8 +55,58 @@ namespace DeclRule
     r.step ⋆
 
   def any_reach (l: List DeclRule): EndoRel PersistentNames :=
-    λ σ σ' ↦ ∃R,
-        R ∈ l.map reach
-      ∧ R σ σ'
+    λ σ σ' ↦
+      ∃ (R: EndoRel PersistentNames),
+          R ∈ l.map reach
+        ∧ R σ σ'
 
 end DeclRule
+
+abbrev Pending    := List Process
+abbrev Persisting := PersistentNames
+
+namespace Program
+  def trigger_all (p: Program) (trig: EphemeralName) (per: Persisting): Pending :=
+    p.reac
+      |>.filter (·.name = trig)
+      |>.filter (·.guard ⊆ per)
+      |>.flatMap (ReactiveRule.effect)
+end Program
+
+namespace Process
+  def exec (p: Process): EndoFun (Pending × Persisting) :=
+    λ (pen, per) ↦ match p with
+      | par   p₁ p₂ => (p₁ :: p₂ :: pen, per)
+      | trig  n     => sorry
+      | add   n     => sorry
+      | rem   n     => sorry
+      | later p     => sorry
+      | halt        => sorry
+end Process
+
+-- Synchronous semantics
+inductive Runto {p: Program}: Rel Pending Persisting where
+  | init: Runto ∅ ∅
+  | fire_where (trig: EphemeralName) pen per:
+      Runto pen per →
+      Runto (pen ++ p.trigger_all trig per) per
+  | eval_where (p: Process) pen per:
+      p ∈ pen →
+      Runto pen per →
+      Runto (pen.erase p) per
+
+
+namespace Process
+  def seq (p₁ p₂: Process) := p₁.par p₂.later
+
+  def seq_list: List Process → Process
+    | [] => Process.halt
+    | p :: l => p.seq (seq_list l)
+end Process
+
+instance: Coe (List Process) Process where
+  coe := Process.seq_list
+
+notation:max a " ∣∣ " b => Process.par a b
+
+example (p₁ p₂ p₃: Process): Process := [p₁ ∣∣ p₂, p₃ ∣∣ [p₁, p₃] ∣∣ p₂]
